steel/Zeta.Steel.ThreadRelDef.fst
@@ -13,4 +13,5 @@ let related_tsm (s: s_thread_state) (i: i_thread_state)
     (i.IV.valid ==>
      ((related_tid s.thread_id i.IV.tid) /\
       (related_timestamp s.clock i.IV.clock) /\
+      (related_base_key s.last_evict_key i.IV.last_evict_key) /\
       (related_store s.store i.IV.st)))
