steel/Zeta.Steel.FormatsManual.fsti
@@ -54,3 +54,4 @@ let eq_value (v0 v1:value)
     | DValue None, DValue None -> true
     | DValue (Some vt0), DValue (Some vt1) -> eq_value_type vt0 vt1
     | _ -> false
+
